added a proof that halve refines the halve_spec

theories/Merge.v
@@ -9,6 +9,8 @@ From ITree Require Export ITree ITreeFacts Eq.Rutt.
 From Paco Require Import paco.
 From Coq Require Export Eqdep EqdepFacts.
 
+Require Export Refinement.
+
 Import Monads.
 Import MonadNotation.
 Local Open Scope monad_scope.
@@ -22,7 +24,195 @@ Inductive sorted : list nat -> Prop :=
   | sorted_singleton x : sorte
 . *)
 
+
+Inductive sorted : list nat -> Prop :=
+  | sorted_nil : sorted nil
+  | sorted_single x : sorted (x :: nil)
+  | sorted_cons x y l : x <= y -> sorted (y :: l) -> sorted (x :: y :: l).
+
+Lemma sorted_tail : forall l x, sorted (x :: l) -> sorted l.
+Proof.
+  intros l. induction l; intros; try (constructor; fail).
+  inv H. auto.
+Qed.
+(*
+Definition list_ind2_principle' (A : Type) (P : list A -> Prop) (Hnil : P nil)
+         (Hcons1 : forall a, P (a :: nil) ) (Hcons2 : forall a b l, P l -> P (a :: b :: l))
+         l : P l :=
+  fix rec l :=
+    match l with
+    | nil => Hnil
+    | a :: nil => Hcons1 a
+    | a :: b :: t => Hcons2 a b t (rec t) end. l.
+*)
+Lemma list_ind2_principle :
+    forall (A : Type) (P : list A -> Prop),
+      P nil ->
+      (forall (a:A), P (a :: nil)) ->
+      (forall (a b : A) (l : list A), P l -> P (a :: b :: l)) ->
+      forall l : list A, P l.
+Proof. 
+  intros. 
+  set (fix rec l := 
+         match l return P l with 
+         | nil => H
+         | a :: nil => H0 a
+         | a :: b :: t => H1 a b t (rec t)
+         end
+      ) as f. auto.
+Qed.
+
 (*rec_fix*)
+
+Definition halve {E} : list nat -> itree E (list nat * list nat) :=
+    rec_fix (fun halve_rec l =>
+               match l with
+               | x :: y :: t => '(l1,l2) <- halve_rec t;; Ret (x :: l1, y :: l2)
+               | x :: nil => Ret ( x :: nil  , nil )
+               | nil => Ret ( nil , nil ) end
+
+).
+
+Definition assert_spec {E} (P : Type) : itree_spec E unit :=
+  trigger (@Spec_exists E P );; Ret tt.
+
+Lemma padded_assert_pad_elim {E1 E2} RE REAns R1 R2 RR P
+      (phi : itree_spec E1 R1) (kphi : unit -> itree_spec E2 R2) :
+  P -> padded_refines RE REAns RR phi (kphi tt) ->
+  padded_refines RE REAns RR phi (ITree.bind (assert_spec P) kphi ).
+Proof.
+  intros. setoid_rewrite bind_trigger.
+  unfold padded_refines in *. rewrite pad_bind, pad_vis.
+  setoid_rewrite pad_ret. rewrite bind_vis. setoid_rewrite bind_tau.
+  setoid_rewrite bind_ret_l. pstep. constructor. auto. constructor. pstep_reverse.
+Qed.
+
+Lemma padded_assert_pad_eliml {E1 E2} RE REAns R1 R2 RR P
+      (phi : itree_spec E1 R1) (kphi : unit -> itree_spec E2 R2) :
+  (P -> padded_refines RE REAns RR (kphi tt) phi) ->
+  padded_refines RE REAns RR (ITree.bind (assert_spec P) kphi ) phi.
+Proof.
+  intros. setoid_rewrite bind_trigger.
+  unfold padded_refines in *. rewrite pad_bind, pad_vis.
+  setoid_rewrite pad_ret. rewrite bind_vis. setoid_rewrite bind_tau.
+  setoid_rewrite bind_ret_l. pstep. constructor. 
+  intros HP. specialize (H HP). constructor. pstep_reverse.
+Qed.
+
+
+Definition assume_spec {E} (P : Type) : itree_spec E unit :=
+  trigger (@Spec_forall E P );; Ret tt.
+
+Lemma padded_assume_pad_elim {E1 E2} RE REAns R1 R2 RR P
+      (phi : itree_spec E1 R1) (kphi : unit -> itree_spec E2 R2) :
+  (P -> padded_refines RE REAns RR phi (kphi tt)) ->
+  padded_refines RE REAns RR phi (ITree.bind (assume_spec P) kphi ).
+Proof.
+  intros. setoid_rewrite bind_trigger.
+  unfold padded_refines in *. rewrite pad_bind, pad_vis.
+  setoid_rewrite pad_ret. rewrite bind_vis. setoid_rewrite bind_tau.
+  setoid_rewrite bind_ret_l. pstep. constructor. 
+  intros HP. specialize (H HP). constructor. pstep_reverse.
+Qed.  
+
+Lemma padded_assume_pad_eliml {E1 E2} RE REAns R1 R2 RR P
+      (phi : itree_spec E1 R1) (kphi : unit -> itree_spec E2 R2) :
+  P -> padded_refines RE REAns RR (kphi tt) phi ->
+  padded_refines RE REAns RR (ITree.bind (assume_spec P) kphi ) phi.
+Proof.
+  intros. setoid_rewrite bind_trigger.
+  unfold padded_refines in *. rewrite pad_bind, pad_vis.
+  setoid_rewrite pad_ret. rewrite bind_vis. setoid_rewrite bind_tau.
+  setoid_rewrite bind_ret_l. pstep. constructor. auto. constructor. pstep_reverse.
+Qed.
+
+Definition spec_exists {E} (T : Type) : itree_spec E T :=
+  trigger (@Spec_exists E T).
+
+
+(**)
+Lemma spec_exists_elim {E1 E2} S1 R2 S2 RE REAns RR (phi : itree_spec E1 S1) 
+      (kphi : R2 -> itree_spec E2 S2 ) r :
+  refines RE REAns RR phi (kphi r) ->
+  refines RE REAns RR phi (ITree.bind (spec_exists R2) kphi ).
+Proof.
+  intros. unfold spec_exists. setoid_rewrite bind_trigger.
+  pstep. econstructor. pstep_reverse.
+Qed.
+
+Opaque assert_spec.
+
+(*maybe there is a simpler way to derive this proof from the previous one*)
+Lemma padded_spec_exists_elim {E1 E2} S1 R2 S2 RE REAns RR (phi : itree_spec E1 S1) 
+      (kphi : R2 -> itree_spec E2 S2 ) r :
+  padded_refines RE REAns RR phi (kphi r) ->
+  padded_refines RE REAns RR phi (ITree.bind (spec_exists R2) kphi ).
+Proof.
+  intros.  unfold padded_refines in *. rewrite pad_bind. setoid_rewrite pad_vis.
+  rewrite bind_vis. 
+  setoid_rewrite pad_ret. setoid_rewrite bind_tau. setoid_rewrite bind_ret_l.
+  pstep. econstructor. Unshelve. all : auto. constructor. pstep_reverse.
+Qed.
+
+Lemma padded_spec_exists_eliml {E1 E2} S1 R2 S2 RE REAns RR (phi : itree_spec E1 S1) 
+      (kphi : R2 -> itree_spec E2 S2 ) :
+  (forall r, padded_refines RE REAns RR (kphi r) phi) ->
+  padded_refines RE REAns RR (ITree.bind (spec_exists R2) kphi ) phi .
+Proof.
+  intros.  unfold padded_refines in *. rewrite pad_bind. setoid_rewrite pad_vis.
+  rewrite bind_vis. 
+  setoid_rewrite pad_ret. setoid_rewrite bind_tau. setoid_rewrite bind_ret_l.
+  pstep. econstructor. intros. constructor. pstep_reverse. apply H.
+Qed.
+
+Ltac existssr a := apply padded_spec_exists_elim with (r := a).
+
+Ltac eexistssr := eapply padded_spec_exists_elim.
+
+Ltac existssl := apply padded_spec_exists_eliml.
+
+
+Definition spec_forall {E} (T : Type) : itree_spec E T :=
+  trigger (@Spec_forall E T).
+
+Lemma spec_forall_elim {E1 E2} S1 R2 S2 RE REAns RR (phi : itree_spec E1 S1) 
+      (kphi : R2 -> itree_spec E2 S2 ) :
+  (forall r, refines RE REAns RR phi (kphi r)) ->
+  refines RE REAns RR phi (ITree.bind (spec_forall R2) kphi ).
+Proof.
+  intros. unfold spec_forall. rewrite bind_trigger.
+  pstep. constructor. intros. pstep_reverse. apply H.
+Qed.
+
+Lemma padded_spec_forall_elim {E1 E2} S1 R2 S2 RE REAns RR (phi : itree_spec E1 S1) 
+      (kphi : R2 -> itree_spec E2 S2 ):
+  (forall r, padded_refines RE REAns RR phi (kphi r)) ->
+  padded_refines RE REAns RR phi (ITree.bind (spec_forall R2) kphi ).
+Proof.
+  intros.  unfold padded_refines in *. rewrite pad_bind. setoid_rewrite pad_vis.
+  rewrite bind_vis. 
+  setoid_rewrite pad_ret. setoid_rewrite bind_tau. setoid_rewrite bind_ret_l.
+  pstep. constructor. intros.  constructor. pstep_reverse.
+  apply H.
+Qed.
+
+Lemma padded_spec_forall_eliml {E1 E2} S1 R2 S2 RE REAns RR (phi : itree_spec E1 S1) 
+      (kphi : R2 -> itree_spec E2 S2 ) r:
+  padded_refines RE REAns RR (kphi r) phi ->
+  padded_refines RE REAns RR (ITree.bind (spec_forall R2) kphi ) phi.
+Proof.
+  intros.  unfold padded_refines in *. rewrite pad_bind. setoid_rewrite pad_vis.
+  rewrite bind_vis. 
+  setoid_rewrite pad_ret. setoid_rewrite bind_tau. setoid_rewrite bind_ret_l.
+  pstep. econstructor. constructor. pstep_reverse.
+Qed.
+
+Definition halve_spec {E} (l : list nat) : itree_spec E (list nat * list nat) :=
+  l1 <- spec_exists (list nat);; 
+  l2 <- spec_exists (list nat);;
+  assert_spec (Permutation l (l1 ++ l2) );;
+  Ret (l1, l2).
+
 Definition merge {E} : (list nat * list nat) -> itree E (list nat) :=
   rec_fix ( fun merge_rec '(l1, l2) =>
               match (l1,l2) with
@@ -36,15 +226,20 @@ Definition merge {E} : (list nat * list nat) -> itree E (list nat) :=
               | (l1, nil) => Ret l1
               | (nil, l2) => Ret l2 end ).
 
-Definition halve {E} : list nat -> itree E (list nat * list nat) :=
-    rec_fix (fun halve_rec l =>
-               match l with
-               | x :: y :: t => '(l1,l2) <- halve_rec l;; Ret (x :: l1, y :: l2)
-               | x :: nil => Ret ( x :: nil  , nil )
-               | nil => Ret ( nil , nil ) end
+Definition merge_spec1 {E} l1 l2 : itree_spec E (list nat) :=
+  l <- spec_exists (list nat);;
+  assert_spec (Permutation l (l1 ++ l2) );;
+  Ret l.
 
-).
+Definition merge_spec2 {E} l1 l2 : itree_spec E (list nat) :=
+  assume_spec (sorted l1);;
+  assume_spec (sorted l2);;
+  l <- spec_exists (list nat);;
+  assert_spec (sorted l);;
+  Ret l.
 
+Definition merge_spec {E} l1 l2 : itree_spec E (list nat) := 
+  and_spec (merge_spec1 l1 l2) (merge_spec2 l1 l2).
 
 (*missing base case*)
 Definition sort {E} : list nat -> itree E (list nat) :=
@@ -58,14 +253,90 @@ Definition sort {E} : list nat -> itree E (list nat) :=
                merge (l1,l2)
           ).
 
+Definition sort_spec {E} (l : list nat) : itree_spec E (list nat) :=
+  l' <- spec_exists (list nat);;
+  assert_spec (Permutation l l');;
+  assert_spec (sorted l');;
+  Ret l'.
+
+
+Definition padded_refines_eq {E R1 R2} RR (phi1 : itree_spec E R1) (phi2 : itree_spec E R2) :=
+  padded_refines eqE eqEAns RR phi1 phi2.
+
+Global Instance padded_refines_eq_refl {E R} : Reflexive (@padded_refines_eq E R R eq).
+Proof.
+  red. intros. unfold padded_refines_eq, padded_refines. apply refl_refines; auto.
+  - red. intros. constructor.
+  - red. intros. inv H. inj_existT. subst. auto.
+  - apply pad_is_padded.
+Qed.
+
+Global Instance padded_refines_eq_trans {E R} : Transitive (@padded_refines_eq E R R eq).
+Proof.
+  intros phi1 phi2 phi3 Hphi12 Hphi23. unfold padded_refines_eq, padded_refines in *.
+  eapply refines_monot; try eapply refinesTrans; eauto with solve_padded; try apply pad_is_padded.
+  - intros. assert (A = B). inv PR. auto. subst.  assert (ea = eb). inv PR. inj_existT.
+    subst. auto. subst. assert (x0 = x1). inv PR. inj_existT. subst. auto.
+    subst. clear PR. constructor. intros. destruct H. inv H. inj_existT. subst.
+    inv H0. inj_existT. subst. exists x1.
+    split; constructor.
+  - intros. inv PR. inj_existT. subst. 
+    assert (A = B0). inv H3. auto. subst. assert (B = B0). inv H4. auto.
+    subst. assert (x0 = e2). inv H3. inj_existT. subst. auto. subst. auto.
+  - intros. inv PR. auto.
+Qed.
 (*
-Fixpoint merge (l1 l2 : list nat) : list nat :=
-  match l1 with
-  | nil => l2
-  | h1 :: t1 => 
-      match l2 with
-      | nil => l1
-      | h2 :: t2 => if Nat.leb h1 h2
-                  then h1 :: merge t1 l2
-                  else h2 :: merge l1 t2 end end.
+Global Instance padded_refines_eq_bind_proper  E1 E2 RE REAns R1 R2 RR : 
+  Proper (padded_refines_eq eq ==> eq ==> @padded_refines E1 E2 R1 R2 RE REAns RR ) ITree.bind.
 *)
+(*from there there is a bit more *)
+
+Lemma interp_mrec_ret : 
+  forall {D E : Type -> Type} (ctx : forall T : Type, D T -> itree (D +' E) T) R (r :R),
+    interp_mrec ctx (Ret r) ≅ Ret r.
+Proof.
+  intros. setoid_rewrite unfold_iter. cbn. rewrite bind_ret_l. reflexivity.
+Qed.
+
+
+Instance perm_eq A : Equivalence (@Permutation A).
+Proof.
+  constructor.
+  - red. apply Permutation_refl.
+  - red. apply Permutation_sym.
+  - red. apply Permutation_trans.
+Qed.
+
+(* in addition to needing more lemmas and stuff, I think I should be careful 
+   about what I am inducting on, its rather subtle*)
+Lemma halve_correct E l : padded_refines_eq eq (halve l) (@halve_spec E l).
+Proof.
+  revert l.
+  apply list_ind2_principle.
+  - unfold halve, halve_spec, rec_fix, rec, mrec. cbn.
+    rewrite interp_mrec_ret. existssr (@nil nat). existssr (@nil nat). 
+    apply padded_assert_pad_elim. constructor. 
+    reflexivity.
+  - intros n. cbn. unfold halve, halve_spec, rec_fix, rec, mrec. cbn.
+    rewrite interp_mrec_ret. existssr ( n :: nil ). existssr (@nil nat).
+    apply padded_assert_pad_elim. cbn. repeat constructor.
+    reflexivity.
+  - intros a b l Hl.
+    unfold halve, halve_spec, rec_fix, rec, mrec. cbn. cbn.
+    rewrite interp_mrec_bind.
+    setoid_rewrite interp_mrec_trigger. cbn.
+    match goal with |- padded_refines_eq eq (ITree.bind ?h _) _ => set h as t end.
+    assert (t = halve l).
+    { unfold halve, rec_fix, rec, t. reflexivity. }
+    rewrite H. clear H t. etransitivity.
+    eapply padded_refines_bind; eauto. intros; subst. destruct r2 as [l1 l2].
+    rewrite interp_mrec_ret. Unshelve. 3 : { apply (fun '(l1,l2) => Ret (a :: l1, b :: l2) ). } cbn. reflexivity.
+    cbn. rewrite bind_bind.
+    existssl. intros l1. setoid_rewrite bind_bind. existssl. intros l2.
+    existssr (a :: l1). existssr (b :: l2). rewrite bind_bind.
+    apply padded_assert_pad_eliml. intros. apply padded_assert_pad_elim.
+    { (* this is a permutation fact *) cbn. rewrite Permutation_app_comm. cbn.
+      rewrite H. rewrite Permutation_app_comm. reflexivity. }
+    rewrite bind_ret_l. reflexivity.
+Qed.
+(*got everything except a single Permutation fact*)
